\begin{answer}
    Fill in the table and calculate the sum $T(n)$ below (do not fill in the grayed-out entries):
\begin{center}    
\begin{tabular}{||c | c | c | c ||}
 \hline
 Line number & \makecell{Number of times \\ the line is performed} & Cost of a single repetition & Total cost of this line \\ [0.5ex]
 \hline\hline
 1 & $\Theta(1)$ & $\Theta(1)$ & $\Theta (1)$  \\
 \hline
 2 & $\Theta(1)$ & $\Theta(1)$ & $\Theta (1)$  \\
 \hline
 3 & $\Theta(1)$ & $\Theta(1)$ & $\Theta (1)$  \\
  \hline
 4 & $\Theta(n)$ & $\Theta(1)$ & $\Theta (n)$  \\
   \hline
 5 & $\Theta(n)$ & $\Theta(1)$ & $\Theta (n)$  \\
  \hline
 6 & $\Theta(n)$ & $\Theta(1)$ & $\Theta (n)$  \\
    \hline
 7 & $\Theta(n)$ & $\Theta(1)$ & $\Theta (n)$  \\
 \hline
 8 & \cellcolor{Gray} & \cellcolor{Gray} & \cellcolor{Gray} \\
 \hline
 9 & \cellcolor{Gray} & \cellcolor{Gray} & \cellcolor{Gray} \\
 \hline
 10 & $\Theta(1)$ & $\Theta(1)$ & $\Theta (1)$  \\
 \hline
 11 & $\Theta(1)$ & $\Theta(1)$ & $\Theta (1)$  \\
 \hline
 12 & $\Theta(1)$ & $\Theta(1)$ & $\Theta (1)$  \\
 \hline
 13 & $\Theta(1)$ & $\Theta(1)$ & $\Theta (1)$  \\
 \hline
 14 & $\Theta(1)$ & $\Theta(1)$ & $\Theta (1)$  \\
 \hline
 15 & \cellcolor{Gray} & \cellcolor{Gray} & \cellcolor{Gray} \\
 \hline
 16 & $\Theta(1)$ & $\Theta(1)$ & $\Theta (1)$  \\
 \hline
 17 & \cellcolor{Gray} & \cellcolor{Gray} & \cellcolor{Gray} \\
 \hline
 18 & \cellcolor{Gray} & \cellcolor{Gray} & \cellcolor{Gray} \\
 \hline
 19 & $\Theta(1)$ & $\Theta(1)$ & $\Theta (1)$  \\
 \hline
 Total & \cellcolor{Gray} & \cellcolor{Gray} & $\Theta (n)$  \\
 \hline
\end{tabular}
\end{center}
\item In the worst case, the "right" element is always the smallest or largest element in the array, leading to a seperation of the array to 2 sub arrays of size 1, and $n - 1$. Which leads to the following time complexity formula:
\[ T(n) = T(n-1) + n \]
\item Proof by induction that $ T(n) \in \theta(n^2)$:
\item induction base: $n = 1$:
\item $ 0 \leq c_1 \cdot 1^2 \leq T(1) = 1 \leq c_2 \cdot 1^2$ so $ c_1 = 1, c_2 = 1$

\item Induction step

\item $T(n) = T(n - 1) - n = T(n-2) + n - 1 +n = T(n - 3) + n- 2 +2n-1 = ... = T(n-i) + i \cdot n - \sum_{k=1}^{i-1} k = T(n-i) + i \cdot n - \frac{i \cdot (i-1)}{2}$
\item We want to find the i that will bring us to T(1) - the stopping condition: $ i = n - 1 $.
\item $T(n) = T(1) + n^2 - n - \frac{n^2}{2} + n + \frac{n}{2} - 1= T(1) + \frac{n^2}{2} + \frac{n}{2} - 1= \theta(1) + \theta(n^2) + \theta(n) = \theta(n^2)$